coq/README.md
@@ -3,4 +3,5 @@ Stlc-comp.v - STLC with computation and value distinction. <br/>
 Stlc-eff.v - STLC-comp with effect annotations. <br/>
 Stlc-algebraiceffects-1op.v - Basic algebraic effects with 1-operation handlers <br/>
 Stlc-algebraiceffects-1op-ops.v - Basic algebraic effects with 1-operation handlers and operations in the types instead of effects<br/>
+Stlc-algebraiceffects-static-instances-1op-ops.v - Basic algebraic effects with 1-operation handlers and static instances<br/>
 
